src/GenLow.v
@@ -28,631 +28,666 @@ Qed.
    tries to follow this code organization/abstraction. We need to
    expose quite a bit on the proof side for this to work though. *)
 Module Type GenLowInterface.
-Parameter G : Type -> Type.
 
-(* Standard (primitive) generator interface *)
-Parameter returnGen  : forall {A : Type}, A -> G A.
-(* TODO: Add dependent combinator *)
-Parameter bindGen :  forall {A B : Type}, G A -> (A -> G B) -> G B.
-(* Parameter bindGen :  forall {A B : Type}, (g : G A) -> ((a : A) -> (_ : a \in semGen g) -> G B) -> G B. *)
-Parameter bindGenOpt : forall {A B : Type}, G (option A) -> (A -> G (option B)) -> G (option B).
-Parameter run  : forall {A : Type}, G A -> nat -> RandomSeed -> A.
-Parameter fmap : forall {A B : Type}, (A -> B) -> G A -> G B.
-Parameter sized : forall {A: Type}, (nat -> G A) -> G A.
-Parameter resize : forall {A: Type}, nat -> G A -> G A.
-Parameter promote : forall {A : Type}, Rose (G A) -> G (Rose A).
-Parameter suchThatMaybe : forall {A : Type}, G A -> (A -> bool) ->
+  (** * Type of generators *)
+
+  Parameter G : Type -> Type.
+
+  (** * Primitive generator combinators *)
+
+  Parameter returnGen  : forall {A : Type}, A -> G A.
+  (* TODO: Add dependent combinator *)
+  Parameter bindGen :  forall {A B : Type}, G A -> (A -> G B) -> G B.
+  (* Parameter bindGen :  forall {A B : Type}, (g : G A) -> ((a : A) -> (_ : a \in semGen g) -> G B) -> G B. *)
+  Parameter bindGenOpt : forall {A B : Type}, G (option A) -> (A -> G (option B)) -> G (option B).
+  Parameter run  : forall {A : Type}, G A -> nat -> RandomSeed -> A.
+  Parameter fmap : forall {A B : Type}, (A -> B) -> G A -> G B.
+  Parameter sized : forall {A: Type}, (nat -> G A) -> G A.
+  Parameter resize : forall {A: Type}, nat -> G A -> G A.
+  Parameter promote : forall {A : Type}, Rose (G A) -> G (Rose A).
+  Parameter suchThatMaybe : forall {A : Type}, G A -> (A -> bool) ->
+                                          G (option A).
+  Parameter suchThatMaybeOpt : forall {A : Type}, G (option A) -> (A -> bool) ->
                                              G (option A).
-Parameter suchThatMaybeOpt : forall {A : Type}, G (option A) -> (A -> bool) ->
-                                                G (option A).
-Parameter choose : forall {A : Type} `{ChoosableFromInterval A}, (A * A) -> G A.
-Parameter sample : forall {A : Type}, G A -> list A.
+  Parameter choose : forall {A : Type} `{ChoosableFromInterval A}, (A * A) -> G A.
+  Parameter sample : forall {A : Type}, G A -> list A.
 
 
-(* LL: The abstraction barrier is annoying :D *)
-Parameter variant : forall {A : Type}, SplitPath -> G A -> G A.
-Parameter reallyUnsafePromote : forall {r A:Type}, (r -> G A) -> G (r -> A).
+  (* LL: The abstraction barrier is annoying :D *)
+  Parameter variant : forall {A : Type}, SplitPath -> G A -> G A.
+  Parameter reallyUnsafePromote : forall {r A:Type}, (r -> G A) -> G (r -> A).
 
-Parameter promoteVariant : forall {A B : Type} (a : A) (f : A -> SplitPath) (g : G B) size 
-                            (r r1 r2 : RandomSeed),
-  randomSplit r = (r1,r2) ->                              
-  run (reallyUnsafePromote (fun a => variant (f a) g)) size r a = 
-  run g size (varySeed (f a) r1).
+  Parameter promoteVariant : forall {A B : Type} (a : A) (f : A -> SplitPath) (g : G B) size 
+                               (r r1 r2 : RandomSeed),
+                               randomSplit r = (r1,r2) ->                              
+                               run (reallyUnsafePromote (fun a => variant (f a) g)) size r a = 
+                               run g size (varySeed (f a) r1).
 
-(* Set of outcomes semantics definitions (repeated below) *)
-Definition semGenSize {A : Type} (g : G A) (size : nat) : set A :=
-  codom (run g size).
-Definition semGen {A : Type} (g : G A) : set A :=
-  \bigcup_size semGenSize g size.
+  (** * Semantics of generators *)
 
-(* Size characterization of generators *)
-(* begin Unsized *)
-Class Unsized {A} (g : G A) := {
-  unsized : forall s1 s2, semGenSize g s1 <--> semGenSize g s2 }.
-(* end Unsized *)
+  (* Set of outcomes semantics definitions (repeated below) *)
+  Definition semGenSize {A : Type} (g : G A) (size : nat) : set A :=
+    codom (run g size).
+  Definition semGen {A : Type} (g : G A) : set A :=
+    \bigcup_size semGenSize g size.
 
-(* begin SizeMonotonic *)
-Class SizeMonotonic {A} (g : G A) := { 
-  monotonic : forall s1 s2, s1 <= s2 -> semGenSize g s1 \subset semGenSize g s2 }.
-(* end SizeMonotonic *)
+  (** * Properties of generators *)
 
-(* TODO: Enhance with properties? *)
-Class CanonicalSize A := 
-  { sizeOf : A -> nat }.
+  (** A generator is [Unsized] if its semantics does not depend on the runtime size *)
+  (* begin Unsized *)
+  Class Unsized {A} (g : G A) :=
+    {
+      unsized : forall s1 s2, semGenSize g s1 <--> semGenSize g s2
+    }.
+  (* end Unsized *)
+  
+  (** Sized generators monotonic in the size parameter *)
+  Class SizedMonotonic {A} (g : nat -> G A) :=
+    {
+      (* TODO remove prime when GenSizedSizeMotonic is modified *)
+      sizeMonotonic' :
+        forall s s1 s2,
+          s1 <= s2 ->
+          semGenSize (g s1) s \subset semGenSize (g s2) s
+    }.
+  
+  (** Generators monotonic in the runtime size parameter *)
+  Class SizeMonotonic {A} (g : G A) :=
+    {
+      monotonic :
+        forall s1 s2, s1 <= s2 -> semGenSize g s1 \subset semGenSize g s2
+    }.
 
-(* Zoe: We do not need that when we do automatic resolution. Changing it to a lemma ? *)
-(* CH: Why does Unsized need a _ when A is marked as implict! *)
-(* begin unsizedMonotonic *)
-Parameter unsizedMonotonic : forall {A} (g : G A), Unsized g -> SizeMonotonic g.
-(* end unsizedMonotonic *)
+  (* CH: Why does Unsized need a _ when A is marked as implict! *)
+  Parameter unsized_alt_def :
+    forall A (g : G A) `{Unsized _ g},
+    forall s, semGenSize g s <--> semGen g.
 
+  (* begin unsizedMonotonic *)
+  Declare Instance unsizedMonotonic : forall {A} (g : G A), Unsized g -> SizeMonotonic g.
+  (* end unsizedMonotonic *)
+  
 
-Parameter unsized_alt_def : 
-  forall A (g : G A) `{Unsized _ g},
-  forall s, semGenSize g s <--> semGen g.
+  (** *  Semantics of combinators *)
+  
+  Parameter semReturn :
+    forall A (x : A), semGen (returnGen x) <--> [set x].
+  Parameter semReturnSize :
+    forall A (x : A) size, semGenSize (returnGen x) size <--> [set x].
+  
+  Declare Instance unsizedReturn {A} (x : A) : Unsized (returnGen x).
+  Declare Instance returnGenSizeMonotonic {A} (x : A) : SizeMonotonic (returnGen x).
 
-(* Set of outcomes characterization of generators *)
-Parameter semReturn :
-  forall A (x : A), semGen (returnGen x) <--> [set x].
-Parameter semReturnSize :
-  forall A (x : A) size, semGenSize (returnGen x) size <--> [set x].
-
-Declare Instance unsizedReturn {A} (x : A) : Unsized (returnGen x).
-Declare Instance returnGenSizeMonotonic {A} (x : A) : SizeMonotonic (returnGen x).
-
-Parameter semBindSize :
-  forall A B (g : G A) (f : A -> G B) (size : nat),
-    semGenSize (bindGen g f) size <-->
-               \bigcup_(a in semGenSize g size) semGenSize (f a) size.
-
-Parameter monad_leftid : 
-  forall {A B : Type} (a: A) (f : A -> G B),
-    semGen (bindGen (returnGen a) f) <--> semGen (f a).
-Parameter monad_rightid : 
-  forall {A : Type} (g : G A),
-    semGen (bindGen g returnGen) <--> semGen g.
-Parameter monad_assoc: 
-  forall {A B C : Type} (ga : G A) (fb : A -> G B) (fc : B -> G C),
-    semGen (bindGen (bindGen ga fb) fc) <--> 
-    semGen (bindGen ga (fun a => bindGen (fb a) fc)).
-
-(* I'm not sure how this universal quantifier will behave *)
-(* begin bindUnsized *)
-Declare Instance bindUnsized {A B} (g : G A) (f : A -> G B)
-    `{Unsized _ g} `{forall x, Unsized (f x)} : Unsized (bindGen g f).
-(* end bindUnsized *)
-
-Declare Instance bindMonotonic
-        {A B} (g : G A) (f : A -> G B)
-        `{SizeMonotonic _ g} `{forall x, SizeMonotonic (f x)} : 
-  SizeMonotonic (bindGen g f).
-
-Parameter semBindUnsized1 :
-  forall A B (g : G A) (f : A -> G B) `{Unsized _ g},
-    semGen (bindGen g f) <--> \bigcup_(a in semGen g) semGen (f a).
-
-Parameter semBindUnsized2 :
-  forall A B (g : G A) (f : A -> G B) `{forall a, Unsized (f a)},
-    semGen (bindGen g f) <--> \bigcup_(a in semGen g) semGen (f a).
-
-Parameter semBindSizeMonotonic :
+  Parameter semBindSize :
+    forall A B (g : G A) (f : A -> G B) (size : nat),
+      semGenSize (bindGen g f) size <-->
+                 \bigcup_(a in semGenSize g size) semGenSize (f a) size.
+  
+  Parameter monad_leftid : 
+    forall {A B : Type} (a: A) (f : A -> G B),
+      semGen (bindGen (returnGen a) f) <--> semGen (f a).
+  Parameter monad_rightid : 
+    forall {A : Type} (g : G A),
+      semGen (bindGen g returnGen) <--> semGen g.
+  Parameter monad_assoc: 
+    forall {A B C : Type} (ga : G A) (fb : A -> G B) (fc : B -> G C),
+      semGen (bindGen (bindGen ga fb) fc) <--> 
+             semGen (bindGen ga (fun a => bindGen (fb a) fc)).
+  
+  (* I'm not sure how this universal quantifier will behave *)
+  (* begin bindUnsized *)
+  Declare Instance bindUnsized {A B} (g : G A) (f : A -> G B)
+          `{Unsized _ g} `{forall x, Unsized (f x)} : Unsized (bindGen g f).
+  (* end bindUnsized *)
+  
+  Declare Instance bindMonotonic
+          {A B} (g : G A) (f : A -> G B)
+          `{SizeMonotonic _ g} `{forall x, SizeMonotonic (f x)} : 
+    SizeMonotonic (bindGen g f).
+  
+  Parameter semBindUnsized1 :
+    forall A B (g : G A) (f : A -> G B) `{Unsized _ g},
+      semGen (bindGen g f) <--> \bigcup_(a in semGen g) semGen (f a).
+  
+  Parameter semBindUnsized2 :
+    forall A B (g : G A) (f : A -> G B) `{forall a, Unsized (f a)},
+      semGen (bindGen g f) <--> \bigcup_(a in semGen g) semGen (f a).
+  
+  Parameter semBindSizeMonotonic :
   forall {A B} (g : G A) (f : A -> G B)
          `{SizeMonotonic _ g} `{forall a, SizeMonotonic (f a)},
     semGen (bindGen g f) <--> \bigcup_(a in semGen g) semGen (f a).
 
-Parameter semFmap :
-  forall A B (f : A -> B) (g : G A),
-    semGen (fmap f g) <--> f @: semGen g.
-Parameter semFmapSize :
-  forall A B (f : A -> B) (g : G A) (size : nat),
-    semGenSize (fmap f g) size <--> f @: semGenSize g size.
+  Parameter semFmap :
+    forall A B (f : A -> B) (g : G A),
+      semGen (fmap f g) <--> f @: semGen g.
 
-Declare Instance fmapUnsized {A B} (f : A -> B) (g : G A) `{Unsized _ g} : 
-  Unsized (fmap f g).
+  Parameter semFmapSize :
+    forall A B (f : A -> B) (g : G A) (size : nat),
+      semGenSize (fmap f g) size <--> f @: semGenSize g size.
 
-Declare Instance fmapMonotonic
-        {A B} (f : A -> B) (g : G A) `{SizeMonotonic _ g} : 
-  SizeMonotonic (fmap f g).
+  Declare Instance fmapUnsized {A B} (f : A -> B) (g : G A) `{Unsized _ g} : 
+    Unsized (fmap f g).
 
-Parameter semChoose :
-  forall A `{ChoosableFromInterval A} (a1 a2 : A), Random.leq a1 a2 ->
-    (semGen (choose (a1,a2)) <-->
-    [set a | Random.leq a1 a && Random.leq a a2]).
+  Declare Instance fmapMonotonic
+          {A B} (f : A -> B) (g : G A) `{SizeMonotonic _ g} : 
+    SizeMonotonic (fmap f g).
 
-Parameter semChooseSize :
-  forall A `{ChoosableFromInterval A} (a1 a2 : A), Random.leq a1 a2 ->
-    forall size, (semGenSize (choose (a1,a2)) size <-->
-    [set a | Random.leq a1 a && Random.leq a a2]).
+  Parameter semChoose :
+    forall A `{ChoosableFromInterval A} (a1 a2 : A),
+      Random.leq a1 a2 ->
+      (semGen (choose (a1,a2)) <--> [set a | Random.leq a1 a && Random.leq a a2]).
 
-Declare Instance chooseUnsized A `{ChoosableFromInterval A} (a1 a2 : A) : 
-  Unsized (choose (a1, a2)).
+  Parameter semChooseSize :
+    forall A `{ChoosableFromInterval A} (a1 a2 : A),
+      Random.leq a1 a2 ->
+      forall size, (semGenSize (choose (a1,a2)) size <-->
+              [set a | Random.leq a1 a && Random.leq a a2]).
 
-Parameter semSized :
-  forall A (f : nat -> G A),
-    semGen (sized f) <--> \bigcup_s semGenSize (f s) s.
+  Declare Instance chooseUnsized A `{ChoosableFromInterval A} (a1 a2 : A) : 
+    Unsized (choose (a1, a2)).
 
-Parameter semSizedSize :
-  forall A (f : nat -> G A) s,
-    semGenSize (sized f) s <--> semGenSize (f s) s.
+  Parameter semSized :
+    forall A (f : nat -> G A),
+      semGen (sized f) <--> \bigcup_s semGenSize (f s) s.
 
-(* TODO change name *)
-Parameter semSized_alt :
-  forall A (f : nat -> G A) `{forall n, SizeMonotonic (f n)},
-    (forall n m s,  n <= m -> semGenSize (f n) s \subset semGenSize (f m) s) ->
-    semGen (sized f) <--> \bigcup_n (semGen (f n)).
+  Parameter semSizedSize :
+    forall A (f : nat -> G A) s,
+      semGenSize (sized f) s <--> semGenSize (f s) s.
 
-Parameter sizedMonotonic :
-  forall A (f : nat -> G A) `{forall n, SizeMonotonic (f n)},
-    (forall n m s,  n <= m -> semGenSize (f n) s \subset semGenSize (f m) s) ->
-    SizeMonotonic (sized f).
+  (* TODO change name *)
 
-Parameter semResize :
-  forall A (n : nat) (g : G A),
-    semGen (resize n g) <--> semGenSize g n.
+  Parameter semSized_alt :
+    forall A (f : nat -> G A) `{forall n, SizeMonotonic (f n)},
+      (forall n m s,  n <= m -> semGenSize (f n) s \subset semGenSize (f m) s) ->
+      semGen (sized f) <--> \bigcup_n (semGen (f n)).
 
-Declare Instance unsizedResize {A} (g : G A) n : 
-  Unsized (resize n g).
+  Declare Instance sizedSizeMonotonic
+          A (gen : nat -> G A) `{forall n, SizeMonotonic (gen n)} `{SizedMonotonic A gen} :
+    SizeMonotonic (sized gen).
+  
+  Parameter semResize :
+    forall A (n : nat) (g : G A),
+      semGen (resize n g) <--> semGenSize g n.
+
+  Declare Instance unsizedResize {A} (g : G A) n : 
+    Unsized (resize n g).
 
 
-(* TODO: We need completeness as well - this is not exact *)
-Parameter semSuchThatMaybe_sound:
-  forall A (g : G A) (f : A -> bool),
-    semGen (suchThatMaybe g f) \subset
-    None |: some @: (semGen g :&: f).
+  (* TODO: We need completeness as well - this is not exact *)
+  Parameter semSuchThatMaybe_sound:
+    forall A (g : G A) (f : A -> bool),
+      semGen (suchThatMaybe g f) \subset None |: some @: (semGen g :&: f).
 
-(* This (very concrete) spec is needed to prove shrinking *)
-Parameter semPromote : forall A (m : Rose (G A)),
-  semGen (promote m) <-->
-  codom2 (fun size seed => fmapRose (fun g => run g size seed) m).
+  (* This (very concrete) spec is needed to prove shrinking *)
+  Parameter semPromote :
+    forall A (m : Rose (G A)),
+      semGen (promote m) <-->
+      codom2 (fun size seed => fmapRose (fun g => run g size seed) m).
 
-Parameter semPromoteSize :
-  forall (A : Type) (m : Rose (G A)) n,
-    semGenSize (promote m) n <-->
-    (fun t : Rose A =>
-       exists (seed : RandomSeed),
-         fmapRose (fun g : G A => run g n seed) m = t).
+  Parameter semPromoteSize :
+    forall (A : Type) (m : Rose (G A)) n,
+      semGenSize (promote m) n <-->
+      (fun t : Rose A =>
+         exists (seed : RandomSeed),
+           fmapRose (fun g : G A => run g n seed) m = t).
 
-(* Those are too concrete, but I need them to prove shrinking.
+  (* Those are too concrete, but I need them to prove shrinking.
    Does this reveal a weakness in our framework?
    Should we try to get rid of this?
    This is expected since the spec of promote is too concrete. *)
 
-Parameter runFmap : forall (A B : Type) (f : A -> B) (g : G A) seed size,
-  run (fmap f g) seed size = f (run g seed size).
+  Parameter runFmap :
+    forall (A B : Type) (f : A -> B) (g : G A) seed size,
+      run (fmap f g) seed size = f (run g seed size).
   
-Parameter runPromote : forall A (m : Rose (G A)) seed size,
-  run (promote m) seed size = fmapRose (fun (g : G A) => run g seed size) m.
-
-Parameter semFmapBind :
-  forall A B C (g : G A) (f1 : B -> C) (f2 : A -> G B),
-    semGen (fmap f1 (bindGen g f2)) <-->
-    semGen (bindGen g (fun x => fmap f1 (f2 x))).
-
+  Parameter runPromote :
+    forall A (m : Rose (G A)) seed size,
+      run (promote m) seed size = fmapRose (fun (g : G A) => run g seed size) m.
+  
+  Parameter semFmapBind :
+    forall A B C (g : G A) (f1 : B -> C) (f2 : A -> G B),
+      semGen (fmap f1 (bindGen g f2)) <-->
+      semGen (bindGen g (fun x => fmap f1 (f2 x))).
+  
 End GenLowInterface.
 
 Module GenLow : GenLowInterface.
 
-(* begin GenType *)
-Inductive GenType (A:Type) : Type := MkGen : (nat -> RandomSeed -> A) -> GenType A.
-(* end GenType *)
+  (** * Type of generators *)
 
-Definition G := GenType.
+  (* begin GenType *)
+  Inductive GenType (A:Type) : Type := MkGen : (nat -> RandomSeed -> A) -> GenType A.
+  (* end GenType *)
+  
+  Definition G := GenType.
 
-(* begin run *)
-Definition run {A : Type} (g : G A) := match g with MkGen f => f end.
-(* end run *)
-
-Definition returnGen {A : Type} (x : A) : G A :=
-  MkGen (fun _ _ => x).
-
-Definition bindGen {A B : Type} (g : G A) (k : A -> G B) : G B :=
-  MkGen (fun n r =>
-           let (r1,r2) := randomSplit r in
-            run (k (run g n r1)) n r2).
-
-Definition bindGenOpt {A B} (g : G (option A)) (f : A -> G (option B)) : G (option B) :=
-  bindGen g (fun ma => 
-  match ma with
-    | None => returnGen None
-    | Some a => f a
-  end).
-
-Definition fmap {A B : Type} (f : A -> B) (g : G A) : G B :=
-  MkGen (fun n r => f (run g n r)).
-
-Definition sized {A : Type} (f : nat -> G A) : G A :=
-  MkGen (fun n r => run (f n) n r).
-
-Definition resize {A : Type} (n : nat) (g : G A) : G A :=
-  match g with
-    | MkGen m => MkGen (fun _ => m n)
-  end.
-
-Definition promote {A : Type} (m : Rose (G A)) : G (Rose A) :=
-  MkGen (fun n r => fmapRose (fun g => run g n r) m).
-
-(* ZP: Split suchThatMaybe into two different functions
+  (** * Primitive generator combinators *)
+  
+  (* begin run *)
+  Definition run {A : Type} (g : G A) := match g with MkGen f => f end.
+  (* end run *)
+  
+  Definition returnGen {A : Type} (x : A) : G A :=
+    MkGen (fun _ _ => x).
+  
+  Definition bindGen {A B : Type} (g : G A) (k : A -> G B) : G B :=
+    MkGen (fun n r =>
+             let (r1,r2) := randomSplit r in
+             run (k (run g n r1)) n r2).
+  
+  Definition bindGenOpt {A B} (g : G (option A)) (f : A -> G (option B)) : G (option B) :=
+    bindGen g (fun ma => 
+                 match ma with
+                   | None => returnGen None
+                   | Some a => f a
+                 end).
+  
+  Definition fmap {A B : Type} (f : A -> B) (g : G A) : G B :=
+    MkGen (fun n r => f (run g n r)).
+  
+  Definition sized {A : Type} (f : nat -> G A) : G A :=
+    MkGen (fun n r => run (f n) n r).
+  
+  Definition resize {A : Type} (n : nat) (g : G A) : G A :=
+    match g with
+      | MkGen m => MkGen (fun _ => m n)
+    end.
+  
+  Definition promote {A : Type} (m : Rose (G A)) : G (Rose A) :=
+    MkGen (fun n r => fmapRose (fun g => run g n r) m).
+  
+  (* ZP: Split suchThatMaybe into two different functions
      to make a proof easier *)
-Definition suchThatMaybeAux {A : Type} (g : G A) (p : A -> bool) :=
-  fix aux (k : nat) (n : nat) : G (option A) :=
-  match n with
-    | O => returnGen None
-    | S n' =>
-      bindGen (resize (2 * k + n) g) (fun x =>
-                                        if p x then returnGen (Some x)
-                                        else aux (S k) n')
-  end.
+  Definition suchThatMaybeAux {A : Type} (g : G A) (p : A -> bool) :=
+    fix aux (k : nat) (n : nat) : G (option A) :=
+    match n with
+      | O => returnGen None
+      | S n' =>
+        bindGen (resize (2 * k + n) g) (fun x =>
+                                          if p x then returnGen (Some x)
+                                          else aux (S k) n')
+    end.
 
-Definition suchThatMaybe {A : Type} (g : G A) (p : A -> bool)
-: G (option A) :=
-  sized (fun x => suchThatMaybeAux g p 0 (max 1 x)).
+  Definition suchThatMaybe {A : Type} (g : G A) (p : A -> bool)
+  : G (option A) :=
+    sized (fun x => suchThatMaybeAux g p 0 (max 1 x)).
 
-Definition suchThatMaybeOptAux {A : Type} (g : G (option A)) (p : A -> bool) :=
-  fix aux (k : nat) (n : nat) : G (option A) :=
-  match n with
-    | O => returnGen None
-    | S n' =>
-      (* What is this 2 * k + n ? *)
-      bindGen (resize (2 * k + n) g) 
-              (fun mx => match mx with 
+  Definition suchThatMaybeOptAux {A : Type} (g : G (option A)) (p : A -> bool) :=
+    fix aux (k : nat) (n : nat) : G (option A) :=
+    match n with
+      | O => returnGen None
+      | S n' =>
+        (* What is this 2 * k + n ? *)
+        bindGen (resize (2 * k + n) g) 
+                (fun mx => match mx with 
                           | Some x => if p x then returnGen (Some x) else (aux (S k) n')
                           | _ => aux (S k) n'
-                         end)
-  end.
+                        end)
+    end.
 
-Definition suchThatMaybeOpt {A : Type} (g : G (option A)) (p : A -> bool)
-: G (option A) := 
-  sized (fun x => suchThatMaybeOptAux g p 0 (max 1 x)).
-
-Fixpoint rnds (rnd : RandomSeed) (n' : nat) : list RandomSeed :=
-  match n' with
-    | O => nil
-    | S n'' =>
-      let (rnd1, rnd2) := randomSplit rnd in
-      cons rnd1 (rnds rnd2 n'')
-  end.
-
-Fixpoint createRange (n : nat) (acc : list nat) : list nat :=
-  match n with
-    | O => List.rev (cons O acc)
-    | S n' => createRange n' (cons n acc)
-  end.
-
-Definition choose {A : Type} `{ChoosableFromInterval A} (range : A * A) : G A :=
-  MkGen (fun _ r => fst (randomR range r)).
-
-Definition sample (A : Type) (g : G A) : list A :=
-  match g with
-    | MkGen m =>
-      let rnd := mkRandomSeed 0 in
-      let l := List.combine (rnds rnd 20) (createRange 10 nil) in
-      List.map (fun (p : RandomSeed * nat) => let (r,n) := p in m n r) l
-  end.
-
-(* LL : Things that need to be in GenLow because of MkGen *)
-
-Definition variant {A : Type} (p : SplitPath) (g : G A) : G A := 
-  match g with 
-    | MkGen f => MkGen (fun n r => f n (varySeed p r))
-  end.
-
-Definition reallyUnsafeDelay {A : Type} : G (G A -> A) :=
-  MkGen (fun r n g => (match g with MkGen f => f r n end)).
-
-Definition reallyUnsafePromote {r A : Type} (m : r -> G A) : G (r -> A) :=
-    (bindGen reallyUnsafeDelay (fun eval => 
-     returnGen (fun r => eval (m r)))).
-
-(* End Things *)
-
-(* Set of outcomes semantics definitions (repeated above) *)
-(* begin semGen *)
-Definition semGenSize {A : Type} (g : G A) (s : nat) : set A := codom (run g s).
-Definition semGen {A : Type} (g : G A) : set A := \bigcup_s semGenSize g s.
-(* end semGen *)
-
+  Definition suchThatMaybeOpt {A : Type} (g : G (option A)) (p : A -> bool)
+  : G (option A) := 
+    sized (fun x => suchThatMaybeOptAux g p 0 (max 1 x)).
   
-(* An important property of generators is size-monotonicity;
-   sized-monotonic generators compose better *)
+  Fixpoint rnds (rnd : RandomSeed) (n' : nat) : list RandomSeed :=
+    match n' with
+      | O => nil
+      | S n'' =>
+        let (rnd1, rnd2) := randomSplit rnd in
+        cons rnd1 (rnds rnd2 n'')
+    end.
+  
+  Fixpoint createRange (n : nat) (acc : list nat) : list nat :=
+    match n with
+      | O => List.rev (cons O acc)
+      | S n' => createRange n' (cons n acc)
+    end.
+  
+  Definition choose {A : Type} `{ChoosableFromInterval A} (range : A * A) : G A :=
+    MkGen (fun _ r => fst (randomR range r)).
+  
+  Definition sample (A : Type) (g : G A) : list A :=
+    match g with
+      | MkGen m =>
+        let rnd := mkRandomSeed 0 in
+        let l := List.combine (rnds rnd 20) (createRange 10 nil) in
+        List.map (fun (p : RandomSeed * nat) => let (r,n) := p in m n r) l
+    end.
+  
+  (* LL : Things that need to be in GenLow because of MkGen *)
+  
+  Definition variant {A : Type} (p : SplitPath) (g : G A) : G A := 
+    match g with 
+      | MkGen f => MkGen (fun n r => f n (varySeed p r))
+    end.
+  
+  Definition reallyUnsafeDelay {A : Type} : G (G A -> A) :=
+    MkGen (fun r n g => (match g with MkGen f => f r n end)).
+  
+  Definition reallyUnsafePromote {r A : Type} (m : r -> G A) : G (r -> A) :=
+    (bindGen reallyUnsafeDelay (fun eval => 
+                                  returnGen (fun r => eval (m r)))).
+  
+  (* End Things *)
 
-Class Unsized {A} (g : G A) := {
-    unsized : forall s1 s2, (semGenSize g s1 <--> semGenSize g s2) }.
+  (** * Semantics of generators *)
 
-Class SizeMonotonic {A} (g : G A) := { 
-    monotonic : 
-      forall s1 s2, s1 <= s2 -> semGenSize g s1 \subset semGenSize g s2 }.
+  (* Set of outcomes semantics definitions (repeated above) *)
+  (* begin semGen *)
+  Definition semGenSize {A : Type} (g : G A) (s : nat) : set A := codom (run g s).
+  Definition semGen {A : Type} (g : G A) : set A := \bigcup_s semGenSize g s.
+  (* end semGen *)
 
-(* TODO: Enhance with properties? *)
-Class CanonicalSize A := 
-  { sizeOf : A -> nat }.
+  (** * Semantic properties of generators *)
 
-(* Unsizedness trivially implies size-monotonicity *)
-Lemma unsizedMonotonic {A} (g : G A) : Unsized g -> SizeMonotonic g. 
-Proof.
-  constructor. intros s1 s2 Hleq.
-  rewrite /unsized /monotonic => a H12.
-    by destruct (unsized s1 s2 a) as [H1 H2]; eauto.
-Qed.
-
-Lemma unsized_alt_def :
-  forall A (g : G A) `{Unsized _ g},
+  Class Unsized {A} (g : G A) :=
+    {
+      unsized : forall s1 s2, semGenSize g s1 <--> semGenSize g s2
+    }.
+  
+  Class SizedMonotonic {A} (g : nat -> G A) :=
+    {
+      (* TODO remove prime when GenSizedSizeMotonic is modified *)
+      sizeMonotonic' :
+        forall s s1 s2,
+          s1 <= s2 ->
+          semGenSize (g s1) s \subset semGenSize (g s2) s
+    }.
+  
+  Class SizeMonotonic {A} (g : G A) :=
+    {
+      monotonic :
+        forall s1 s2, s1 <= s2 -> semGenSize g s1 \subset semGenSize g s2
+    }.
+  
+  (* Unsizedness trivially implies size-monotonicity *)
+  Lemma unsizedMonotonic {A} (g : G A) : Unsized g -> SizeMonotonic g. 
+  Proof.
+    constructor. intros s1 s2 Hleq.
+    rewrite /unsized /monotonic => a H12.
+      by destruct (unsized s1 s2 a) as [H1 H2]; eauto.
+  Qed.
+  
+  Lemma unsized_alt_def :
+    forall A (g : G A) `{Unsized _ g},
     forall s, semGenSize g s <--> semGen g.
-Proof.
-  move => A f H s a. split.
-  move => H'. exists s. split; auto => //.
-  move => [s' [_ H']]. eapply unsized; eauto.
-Qed.
+  Proof.
+    move => A f H s a. split.
+    move => H'. exists s. split; auto => //.
+    move => [s' [_ H']]. eapply unsized; eauto.
+  Qed.
 
-(* begin semReturn *)
-Lemma semReturn {A} (x : A) : semGen (returnGen x) <--> [set x].
-(* end semReturn *)
-Proof.
-  rewrite /semGen /semGenSize /= bigcup_const ?codom_const //.
-          exact: randomSeed_inhabited.
-    by do 2! constructor.
-Qed.
+  (** * Semantics of combinators *)
 
-(* begin semReturnSize *)
-Lemma semReturnSize A (x : A) (s : nat) :
+  (* begin semReturn *)
+  Lemma semReturn {A} (x : A) : semGen (returnGen x) <--> [set x].
+  (* end semReturn *)
+  Proof.
+    rewrite /semGen /semGenSize /= bigcup_const ?codom_const //.
+            exact: randomSeed_inhabited.
+      by do 2! constructor.
+  Qed.
+  
+  (* begin semReturnSize *)
+  Lemma semReturnSize A (x : A) (s : nat) :
   semGenSize (returnGen x) s <--> [set x].
-(* end semReturnSize *)
-Proof.
-by rewrite /semGenSize /= codom_const //; apply: randomSeed_inhabited.
-Qed.
-
-Program Instance unsizedReturn {A} (x : A) : Unsized (returnGen x).
-Next Obligation.
-  by rewrite ! semReturnSize; split; auto.
-Qed.
-
-Instance returnGenSizeMonotonic {A} (x : A) : SizeMonotonic (returnGen x).
-Proof.
-  firstorder.
-Qed.
-
-(* begin semBindSize *)
-Lemma semBindSize A B (g : G A) (f : A -> G B) (s : nat) :
-  semGenSize (bindGen g f) s <-->
-  \bigcup_(a in semGenSize g s) semGenSize (f a) s.
-(* end semBindSize *)
-Proof.
-rewrite /semGenSize /bindGen /= bigcup_codom -curry_codom2l.
-by rewrite -[codom (prod_curry _)]imsetT -randomSplit_codom -codom_comp.
-Qed.
-
-Lemma monad_leftid A B (a : A) (f : A -> G B) :
-  semGen (bindGen (returnGen a) f) <--> semGen (f a).
-Proof.
-by apply: eq_bigcupr => size; rewrite semBindSize semReturnSize bigcup_set1.
-Qed.
-
-Lemma monad_rightid A (g : G A) : semGen (bindGen g returnGen) <--> semGen g.
-Proof.
-apply: eq_bigcupr => size; rewrite semBindSize.
-by rewrite (eq_bigcupr _ (fun x => semReturnSize x size))
-           /semGenSize bigcup_codom codomE.
-Qed.
-
-Lemma monad_assoc A B C (ga : G A) (fb : A -> G B) (fc : B -> G C) :
-  semGen (bindGen (bindGen ga fb) fc) <--> 
-  semGen (bindGen ga (fun a => bindGen (fb a) fc)).
-Proof.
-  apply eq_bigcupr => ?; rewrite !semBindSize ?bigcup_flatten.
+  (* end semReturnSize *)
+  Proof.
+      by rewrite /semGenSize /= codom_const //; apply: randomSeed_inhabited.
+  Qed.
+  
+  Program Instance unsizedReturn {A} (x : A) : Unsized (returnGen x).
+  Next Obligation.
+      by rewrite ! semReturnSize; split; auto.
+  Qed.
+  
+  Instance returnGenSizeMonotonic {A} (x : A) : SizeMonotonic (returnGen x).
+  Proof.
+    firstorder.
+  Qed.
+  
+  (* begin semBindSize *)
+  Lemma semBindSize A B (g : G A) (f : A -> G B) (s : nat) :
+    semGenSize (bindGen g f) s <-->
+               \bigcup_(a in semGenSize g s) semGenSize (f a) s.
+  (* end semBindSize *)
+  Proof.
+    rewrite /semGenSize /bindGen /= bigcup_codom -curry_codom2l.
+      by rewrite -[codom (prod_curry _)]imsetT -randomSplit_codom -codom_comp.
+  Qed.
+  
+  Lemma monad_leftid A B (a : A) (f : A -> G B) :
+    semGen (bindGen (returnGen a) f) <--> semGen (f a).
+  Proof.
+      by apply: eq_bigcupr => size; rewrite semBindSize semReturnSize bigcup_set1.
+  Qed.
+  
+  Lemma monad_rightid A (g : G A) : semGen (bindGen g returnGen) <--> semGen g.
+  Proof.
+    apply: eq_bigcupr => size; rewrite semBindSize.
+      by rewrite (eq_bigcupr _ (fun x => semReturnSize x size))
+                 /semGenSize bigcup_codom codomE.
+  Qed.
+  
+  Lemma monad_assoc A B C (ga : G A) (fb : A -> G B) (fc : B -> G C) :
+    semGen (bindGen (bindGen ga fb) fc) <--> 
+    semGen (bindGen ga (fun a => bindGen (fb a) fc)).
+  Proof.
+    apply eq_bigcupr => ?; rewrite !semBindSize ?bigcup_flatten.
     by apply eq_bigcupr => ?; rewrite !semBindSize ?bigcup_flatten.
-Qed.
+  Qed.
 
-Program Instance bindUnsized
-        {A B} (g : G A) (f : A -> G B) `{Unsized _ g} `{forall x, Unsized (f x)} : 
-  Unsized (bindGen g f).
-Next Obligation.
-  rewrite !semBindSize !unsized_alt_def. move => b. 
-  split; move => [a [H1 H2]]; exists a; split => //; by eapply unsized; eauto.
-Qed.
-
-Program Instance bindMonotonic
-        {A B} (g : G A) (f : A -> G B) `{SizeMonotonic _ g} `{forall x, SizeMonotonic (f x)} : 
-  SizeMonotonic (bindGen g f).
-Next Obligation.
-  rewrite !semBindSize. move => b.
-  move => [a [H3 H4]]; exists a; split => //; eapply monotonic; eauto.
-Qed.
-
-(* begin semBindUnsized1 *)
-Lemma semBindUnsized1 {A B} (g : G A) (f : A -> G B) `{H : Unsized _ g}:
+  Program Instance bindUnsized
+          {A B} (g : G A) (f : A -> G B) `{Unsized _ g} `{forall x, Unsized (f x)} : 
+    Unsized (bindGen g f).
+  Next Obligation.
+    rewrite !semBindSize !unsized_alt_def. move => b. 
+    split; move => [a [H1 H2]]; exists a; split => //; by eapply unsized; eauto.
+  Qed.
+  
+  Program Instance bindMonotonic
+          {A B} (g : G A) (f : A -> G B) `{SizeMonotonic _ g} `{forall x, SizeMonotonic (f x)} : 
+    SizeMonotonic (bindGen g f).
+  Next Obligation.
+    rewrite !semBindSize. move => b.
+    move => [a [H3 H4]]; exists a; split => //; eapply monotonic; eauto.
+  Qed.
+  
+  (* begin semBindUnsized1 *)
+  Lemma semBindUnsized1 {A B} (g : G A) (f : A -> G B) `{H : Unsized _ g}:
     semGen (bindGen g f) <--> \bigcup_(a in semGen g) semGen (f a).
-(* end semBindUnsized1 *)
-Proof.
-  rewrite /semGen. setoid_rewrite semBindSize.
-  setoid_rewrite (@unsized_alt_def A g H). move => b. split.
-  - intros [s [_ [a [H1 H2]]]].
-    exists a. split; exists s; split; by [].
-  - intros [a [[s1 [_ H1]] [s2 [_ H2]]]]. 
-    exists s2. split; first by [].
-    exists a. split; by [].
-Qed.
+  (* end semBindUnsized1 *)
+  Proof.
+    rewrite /semGen. setoid_rewrite semBindSize.
+    setoid_rewrite (@unsized_alt_def A g H). move => b. split.
+    - intros [s [_ [a [H1 H2]]]].
+      exists a. split; exists s; split; by [].
+    - intros [a [[s1 [_ H1]] [s2 [_ H2]]]]. 
+      exists s2. split; first by [].
+      exists a. split; by [].
+  Qed.
+  
+  Lemma semBindUnsized2 :
+    forall A B (g : G A) (f : A -> G B),
+      (forall a, Unsized (f a)) ->
+      semGen (bindGen g f) <--> \bigcup_(a in semGen g) semGen (f a).
+  Proof.
+    move=> A B g f H.
+    rewrite /semGen. setoid_rewrite semBindSize.
+    intro b. split.
+    - intros [s [_ [a [H1 H2]]]].
+      exists a. split; exists s; split => //. 
+    - intros [a [[s1 [_ H1]] [s2 [_  H2]]]].
+      exists s1. split; first by []. exists a. 
+      split; first by []; apply unsized_alt_def; eauto.
+        by eapply unsized_alt_def; eauto.
+  Qed.
 
-Lemma semBindUnsized2 :
-  forall A B (g : G A) (f : A -> G B),
-    (forall a, Unsized (f a)) ->
+  (* begin semBindSizeMonotonic *)
+  Lemma semBindSizeMonotonic {A B} (g : G A) (f : A -> G B)
+        `{Hg : SizeMonotonic _ g} `{Hf : forall a, SizeMonotonic (f a)} :
     semGen (bindGen g f) <--> \bigcup_(a in semGen g) semGen (f a).
-Proof.
-  move=> A B g f H.
-  rewrite /semGen. setoid_rewrite semBindSize.
-  intro b. split.
-  - intros [s [_ [a [H1 H2]]]].
-    exists a. split; exists s; split => //. 
-  - intros [a [[s1 [_ H1]] [s2 [_  H2]]]].
-    exists s1. split; first by []. exists a. 
-    split; first by []; apply unsized_alt_def; eauto.
-    by eapply unsized_alt_def; eauto.
-Qed.
+  (* end semBindSizeMonotonic *)
+  Proof.
+    rewrite /semGen. setoid_rewrite semBindSize.
+    intro b. split.
+    - intros [s [_ [a [H1 H2]]]].
+      exists a. split; exists s; (split; first (compute; by []); first by[]).
+    - intros [a [[s1 [_ H1]] [s2 [_ H2]]]]. exists (max s1 s2).
+      split; first (compute; by []).
+      exists a. split.
+      eapply Hg; last eassumption. by apply/leP; apply Max.le_max_l.
+      eapply Hf; last eassumption. by apply/leP; apply Max.le_max_r.
+  Qed.
 
-(* begin semBindSizeMonotonic *)
-Lemma semBindSizeMonotonic {A B} (g : G A) (f : A -> G B)
-      `{Hg : SizeMonotonic _ g} `{Hf : forall a, SizeMonotonic (f a)} :
-    semGen (bindGen g f) <--> \bigcup_(a in semGen g) semGen (f a).
-(* end semBindSizeMonotonic *)
-Proof.
-  rewrite /semGen. setoid_rewrite semBindSize.
-  intro b. split.
-  - intros [s [_ [a [H1 H2]]]].
-    exists a. split; exists s; (split; first (compute; by []); first by[]).
-  - intros [a [[s1 [_ H1]] [s2 [_ H2]]]]. exists (max s1 s2).
-    split; first (compute; by []).
-    exists a. split.
-    eapply Hg; last eassumption. by apply/leP; apply Max.le_max_l.
-    eapply Hf; last eassumption. by apply/leP; apply Max.le_max_r.
-Qed.
-
-
-Lemma semFmapSize A B (f : A -> B) (g : G A) (size : nat) :
-  semGenSize (fmap f g) size <--> f @: semGenSize g size.
-Proof. by rewrite /fmap /semGenSize /= codom_comp. Qed.
-
-Lemma semFmap A B (f : A -> B) (g : G A) :
-  semGen (fmap f g) <--> f @: semGen g.
-Proof.
-  by rewrite imset_bigcup /semGen (eq_bigcupr _ (semFmapSize _ _)).
-Qed.
-
-Program Instance fmapUnsized {A B} (f : A -> B) (g : G A) `{Unsized _ g} : 
-  Unsized (fmap f g).
-Next Obligation.
-  rewrite !semFmapSize. move => b.
-  by split; move => [a [H1 <-]]; eexists; split; eauto => //; eapply unsized; eauto.
-Qed.
-
-Program Instance fmapMonotonic
-        {A B} (f : A -> B) (g : G A) `{SizeMonotonic _ g} : 
-  SizeMonotonic (fmap f g).
-Next Obligation.
-  rewrite !semFmapSize. move => b.
-  move => [a [H1 <-]]; eexists; split; eauto => //; eapply monotonic; eauto.
-Qed.
-
-
-Lemma semChooseSize A `{ChoosableFromInterval A} (a1 a2 : A) :
-  Random.leq a1 a2 ->
+  Lemma semFmapSize A B (f : A -> B) (g : G A) (size : nat) :
+    semGenSize (fmap f g) size <--> f @: semGenSize g size.
+  Proof.
+      by rewrite /fmap /semGenSize /= codom_comp.
+  Qed.
+  
+  Lemma semFmap A B (f : A -> B) (g : G A) :
+    semGen (fmap f g) <--> f @: semGen g.
+  Proof.
+      by rewrite imset_bigcup /semGen (eq_bigcupr _ (semFmapSize _ _)).
+  Qed.
+  
+  Program Instance fmapUnsized {A B} (f : A -> B) (g : G A) `{Unsized _ g} : 
+    Unsized (fmap f g).
+  Next Obligation.
+    rewrite !semFmapSize. move => b.
+      by split; move => [a [H1 <-]]; eexists; split; eauto => //; eapply unsized; eauto.
+  Qed.
+  
+  Program Instance fmapMonotonic
+          {A B} (f : A -> B) (g : G A) `{SizeMonotonic _ g} : 
+    SizeMonotonic (fmap f g).
+  Next Obligation.
+    rewrite !semFmapSize. move => b.
+    move => [a [H1 <-]]; eexists; split; eauto => //; eapply monotonic; eauto.
+  Qed.
+  
+  Lemma semChooseSize A `{ChoosableFromInterval A} (a1 a2 : A) :
+    Random.leq a1 a2 ->
     forall size, semGenSize (choose (a1,a2)) size <-->
-    [set a | Random.leq a1 a && Random.leq a a2].
-Proof. by move=> /= le_a1a2 m n; rewrite (randomRCorrect n a1 a2). Qed.
+                       [set a | Random.leq a1 a && Random.leq a a2].
+  Proof. by move=> /= le_a1a2 m n; rewrite (randomRCorrect n a1 a2). Qed.
+  
+  Program Instance chooseUnsized {A} `{ChoosableFromInterval A} (a1 a2 : A) : 
+    Unsized (choose (a1, a2)).
+  Next Obligation. by []. Qed.
+  
+  Lemma semChoose A `{ChoosableFromInterval A} (a1 a2 : A) :
+    Random.leq a1 a2 ->
+    (semGen (choose (a1,a2)) <--> [set a | Random.leq a1 a && Random.leq a a2]).
+  Proof. 
+    move=> /= le_a1a2. rewrite <- (unsized_alt_def 1).
+    move => m /=. rewrite (randomRCorrect m a1 a2) //.
+  Qed.
 
-Program Instance chooseUnsized {A} `{ChoosableFromInterval A} (a1 a2 : A) : 
-  Unsized (choose (a1, a2)).
-Next Obligation. by []. Qed.
+  Lemma semSized A (f : nat -> G A) :
+    semGen (sized f) <--> \bigcup_n semGenSize (f n) n.
+  Proof. by []. Qed.
 
-Lemma semChoose A `{ChoosableFromInterval A} (a1 a2 : A) : Random.leq a1 a2 ->
-  (semGen (choose (a1,a2)) <-->
-  [set a | Random.leq a1 a && Random.leq a a2]).
-Proof. 
-  move=> /= le_a1a2. rewrite <- (unsized_alt_def 1).
-  move => m /=. rewrite (randomRCorrect m a1 a2) //.
-Qed.
+  Lemma semSizedSize A(f:nat->G A)s : semGenSize (sized f) s <--> semGenSize (f s) s.
+  Proof. by []. Qed.
+  
+  Lemma semSized_alt A (f : nat -> G A) (H : forall n, SizeMonotonic (f n))
+        (H' : forall n m s,  n <= m -> semGenSize (f n) s \subset semGenSize (f m) s) :
+    semGen (sized f) <--> \bigcup_n (semGen (f n)).
+  Proof.
+    rewrite semSized.
+    move => x; split.
+    - move => [n [HT Hs]].
+      eexists. split; eauto. eexists; eauto.
+    - move => [n [HT [m [_ Hs]]]].
+      eapply semSized. eexists (m + n).
+      split. constructor. 
+      eapply (H' n). ssromega.
+      eapply (H n); try eassumption. ssromega.
+  Qed.
 
-Lemma semSized A (f : nat -> G A) :
-  semGen (sized f) <--> \bigcup_n semGenSize (f n) n.
-Proof. by []. Qed.
+  Instance sizedSizeMonotonic
+           A (gen : nat -> G A) `{forall n, SizeMonotonic (gen n)} `{SizedMonotonic A gen} :
+    SizeMonotonic (sized gen).
+  Proof.
+    constructor. move => s1 s2 Hleq a /semSizedSize H1.
+    eapply semSizedSize.
+    eapply H. eassumption.
+    eapply H0; eassumption.
+  Qed.    
+  
+  Lemma semResize A n (g : G A) : semGen (resize n g) <--> semGenSize g n .
+  Proof.
+      by case: g => g; rewrite /semGen /semGenSize /= bigcup_const.
+  Qed.
+  
+  Program Instance unsizedResize {A} (g : G A) n : 
+    Unsized (resize n g).
+  Next Obligation.
+    rewrite /Unsized /resize /semGenSize.
+    destruct g; split; auto.
+  Qed.
+  
+  Lemma semGenSuchThatMaybeAux_sound {A} :
+    forall g p k n (a : A) size seed,
+      run (suchThatMaybeAux g p k n) size seed = Some a ->
+      a \in semGen g :&: p.
+  Proof.
+    case=> g p k n; elim: n k =>  [//=| n IHn] k a size seed /=.
+    case: (randomSplit seed) => r1 r2; case: ifP=> [/= ? [<-]|_]; last exact: IHn.
+      by split=> //; exists (2 * k + n.+1); split=> //; exists r1.
+  Qed.
 
-Lemma semSizedSize A(f:nat->G A)s : semGenSize (sized f) s <--> semGenSize (f s) s.
-Proof. by []. Qed.
+  (* Not an exact spec !!! *)
+  Lemma semSuchThatMaybe_sound A (g : G A) (f : A -> bool) :
+    semGen (suchThatMaybe g f) \subset
+           None |: some @: (semGen g :&: f).
+  Proof.
+    case=> [a [size [_ [x run_x]]] | ]; last by left.
+    by right; exists a; split=> //; apply: (semGenSuchThatMaybeAux_sound run_x).
+  Qed.
+  
+  Lemma promoteVariant :
+    forall {A B : Type} (a : A) (f : A -> SplitPath) (g : G B) size
+      (r r1 r2 : RandomSeed),
+      randomSplit r = (r1, r2) ->
+      run (reallyUnsafePromote (fun a => variant (f a) g)) size r a = 
+      run g size (varySeed (f a) r1).
+  Proof. 
+    move => A B a p g size r r1 r2 H.
+    rewrite /reallyUnsafePromote /variant.
+    destruct g. rewrite /= H. by [].
+  Qed.
 
-Lemma semSized_alt A (f : nat -> G A) (H : forall n, SizeMonotonic (f n))
-      (H' : forall n m s,  n <= m -> semGenSize (f n) s \subset semGenSize (f m) s) :
-  semGen (sized f) <--> \bigcup_n (semGen (f n)).
-Proof.
-  rewrite semSized.
-  move => x; split.
-  - move => [n [HT Hs]].
-    eexists. split; eauto. eexists; eauto.
-  - move => [n [HT [m [_ Hs]]]].
-    eapply semSized. eexists (m + n).
-    split. constructor. 
-    eapply (H' n). ssromega.
-    eapply (H n); try eassumption. ssromega.
-Qed.
+  Lemma semPromote A (m : Rose (G A)) :
+    semGen (promote m) <-->
+    codom2 (fun size seed => fmapRose (fun g => run g size seed) m).
+  Proof. by rewrite /codom2 curry_codom2l. Qed.
 
-Lemma sizedMonotonic A (f : nat -> G A) (H : forall n, SizeMonotonic (f n))
-      (H' : forall n m s,  n <= m -> semGenSize (f n) s \subset semGenSize (f m) s) :
-  SizeMonotonic (sized f).
-Proof.
-  constructor. move => s1 s2 Hleq a /semSizedSize H1.
-  eapply semSizedSize.
-  eapply H. eassumption.
-  eapply H'; eassumption.
-Qed.
+  Lemma semPromoteSize (A : Type) (m : Rose (G A)) n :
+    semGenSize (promote m) n <-->
+               codom (fun seed => fmapRose (fun g => run g n seed) m).
+  Proof. by []. Qed.
 
-Lemma semResize A n (g : G A) : semGen (resize n g) <--> semGenSize g n .
-Proof.
-by case: g => g; rewrite /semGen /semGenSize /= bigcup_const.
-Qed.
-
-Program Instance unsizedResize {A} (g : G A) n : 
-  Unsized (resize n g).
-Next Obligation.
-  rewrite /Unsized /resize /semGenSize.
-  destruct g; split; auto.
-Qed.
-
-Lemma semGenSuchThatMaybeAux_sound {A} : forall g p k n (a : A) size seed,
-  run (suchThatMaybeAux g p k n) size seed = Some a ->
-  a \in semGen g :&: p.
-Proof.
-case=> g p k n; elim: n k =>  [//=| n IHn] k a size seed /=.
-case: (randomSplit seed) => r1 r2; case: ifP=> [/= ? [<-]|_]; last exact: IHn.
-by split=> //; exists (2 * k + n.+1); split=> //; exists r1.
-Qed.
-
-(* Not an exact spec !!! *)
-Lemma semSuchThatMaybe_sound A (g : G A) (f : A -> bool) :
-  semGen (suchThatMaybe g f) \subset
-  None |: some @: (semGen g :&: f).
-Proof.
-case=> [a [size [_ [x run_x]]] | ]; last by left.
-by right; exists a; split=> //; apply: (semGenSuchThatMaybeAux_sound run_x).
-Qed.
-
-Lemma promoteVariant : forall {A B : Type} (a : A) (f : A -> SplitPath) (g : G B) size
-  (r r1 r2 : RandomSeed), randomSplit r = (r1, r2) ->
-  run (reallyUnsafePromote (fun a => variant (f a) g)) size r a = 
-  run g size (varySeed (f a) r1).
-Proof. 
-  move => A B a p g size r r1 r2 H.
-  rewrite /reallyUnsafePromote /variant.
-  destruct g. rewrite /= H. by [].
-Qed.
-
-Lemma semPromote A (m : Rose (G A)) :
-  semGen (promote m) <-->
-  codom2 (fun size seed => fmapRose (fun g => run g size seed) m).
-Proof. by rewrite /codom2 curry_codom2l. Qed.
-
-Lemma semPromoteSize (A : Type) (m : Rose (G A)) n :
-  semGenSize (promote m) n <-->
-  codom (fun seed => fmapRose (fun g => run g n seed) m).
-Proof. by []. Qed.
-
-(* These are too concrete, but I need them to prove shrinking.
-   Does this reveal a weakness in our framework?
-   Should we try to get rid of this?
-   This is expected since the spec of promote is too concrete.
- *)
-Lemma runFmap (A B : Type) (f : A -> B) (g : G A) seed size :
-  run (fmap f g) seed size = f (run g seed size).
-Proof. by []. Qed.
-
-Lemma runPromote A (m : Rose (G A)) seed size :
-  run (promote m) seed size = fmapRose (fun (g : G A) => run g seed size) m.
-Proof. by []. Qed.
-
-Lemma semFmapBind :
-  forall A B C (g : G A) (f1 : B -> C) (f2 : A -> G B),
-    semGen (fmap f1 (bindGen g f2)) <-->
-    semGen (bindGen g (fun x => fmap f1 (f2 x))).
-Proof.
-  intros. rewrite /semGen. setoid_rewrite semFmapSize.
-  setoid_rewrite semBindSize.
-  apply eq_bigcupr => s. setoid_rewrite semFmapSize.
-  rewrite imset_bigcup. reflexivity.
-Qed.
-
+  Lemma runFmap (A B : Type) (f : A -> B) (g : G A) seed size :
+    run (fmap f g) seed size = f (run g seed size).
+  Proof. by []. Qed.
+  
+  Lemma runPromote A (m : Rose (G A)) seed size :
+    run (promote m) seed size = fmapRose (fun (g : G A) => run g seed size) m.
+  Proof. by []. Qed.
+  
+  Lemma semFmapBind :
+    forall A B C (g : G A) (f1 : B -> C) (f2 : A -> G B),
+      semGen (fmap f1 (bindGen g f2)) <-->
+      semGen (bindGen g (fun x => fmap f1 (f2 x))).
+  Proof.
+    intros. rewrite /semGen. setoid_rewrite semFmapSize.
+    setoid_rewrite semBindSize.
+    apply eq_bigcupr => s. setoid_rewrite semFmapSize.
+    rewrite imset_bigcup. reflexivity.
+  Qed.
+  
 End GenLow.
